compiler/backend/proofs/flat_elimProofScript.sml
@@ -551,7 +551,9 @@ Proof
     \\ gvs [semanticPrimitivesTheory.do_arith_def, AllCaseEqs()]
     \\ simp [do_app_def, semanticPrimitivesTheory.do_arith_def,
               find_sem_prim_res_globals_def, find_result_globals_def,
-              find_v_globals_def, v_has_Eval_def, div_exn_v_def, v_to_flat_def])
+              find_v_globals_def, v_has_Eval_def, div_exn_v_def, v_to_flat_def]
+    \\ rw [find_v_globals_def, v_has_Eval_def,
+           semanticPrimitivesTheory.Boolv_def, v_to_flat_def, Boolv_def])
   \\ Cases_on ‘∃ty1 ty2. op = FromTo ty1 ty2’ >- (
     fs [do_app_def]
     \\ gvs [AllCaseEqs()]
