compiler/backend/semantics/closPropsScript.sml
@@ -2356,6 +2356,16 @@ Proof
     \\ rpt (IF_CASES_TAC \\ gvs [] \\ res_tac)
     \\ gvs []
     \\ gvs [simple_val_rel_def,Boolv_def])
+  \\ Cases_on `∃test. opp = BlockOp BoolNot`
+  >-
+   (gvs [do_app_def] \\ rw []
+    \\ gvs [simple_val_rel_def,Boolv_def]
+    \\ rename [‘LIST_REL _ xs ys’] \\ Cases_on ‘xs’ \\ gvs []
+    \\ rename [‘LIST_REL _ xs ys’] \\ Cases_on ‘xs’ \\ gvs []
+    \\ rw []
+    \\ gvs [backend_commonTheory.true_tag_def,
+            backend_commonTheory.false_tag_def] \\ rfs []
+    \\ Cases_on ‘y’ \\ gvs [] \\ res_tac \\ fs [isClos_def])
   \\ Cases_on `∃ws test. opp = WordOp (WordTest ws test)`
   >-
    (gvs []
